splice hastp

dev2015/dot-smallstep4.v
@@ -155,7 +155,7 @@ Inductive has_type : tenv -> venv -> tm -> ty -> nat -> Prop :=
       has_type GH G1 (tvar true x) T (S n1)
   | T_Vary : forall G1 GH x T n1,
       index x GH = Some T ->
-      closed (length GH) (length G1) 0 T -> 
+      closed (S x) (length G1) 0 T ->
       has_type GH G1 (tvar false x) T (S n1)
   | T_VarPack : forall GH G1 b x T1 T1' n1,
       has_type GH G1 (tvar b x) T1' n1 ->
@@ -708,7 +708,7 @@ Proof.
   - eapply closed_upgrade_gh. eapply IHS2. eauto. omega. rewrite H4. rewrite app_length. omega. 
   (* has_type *)
   - subst. eapply closed_upgrade_gh. eauto. omega.
-  - eauto.
+  - subst. eapply closed_upgrade_gh. eauto. eapply index_max. eauto.
   - econstructor. eapply closed_upgrade_gh. eauto. omega.
   - eapply IHT in H1. inversion H1; subst. eauto. omega.
   - econstructor. eauto.
@@ -1542,6 +1542,44 @@ Proof.
   rewrite <- splice_open_permute. reflexivity.
 Qed.
 
+Lemma splice_open_permute_lex: forall {X} (G:list X) T x j,
+  length G <= x ->
+  splice (length G) (open j (TVar false x) T) =
+  open j (TVar false (x + 1)) (splice (length G) T).
+Proof.
+  intros X G T x j LE. generalize dependent j. induction T; intros; simpl; eauto;
+  try rewrite IHT1; try rewrite IHT2; try rewrite IHT; eauto.
+  destruct b; eauto.
+  case_eq (beq_nat j i); intros E; simpl; eauto.
+  unfold splice_var.
+  case_eq (le_lt_dec (length G) x); intros LE1 E1; eauto.
+  omega.
+Qed.
+
+Lemma splice_open_permute_xgt: forall {X} (G:list X) T x j,
+   x < length G ->
+   splice (length G) (open j (TVar false x) T) =
+   open j (TVar false x) (splice (length G) T).
+Proof.
+  intros X G T x j LE. generalize dependent j. induction T; intros; simpl; eauto;
+  try rewrite IHT1; try rewrite IHT2; try rewrite IHT; eauto.
+  destruct b; eauto.
+  case_eq (beq_nat j i); intros E; simpl; eauto.
+  unfold splice_var.
+  case_eq (le_lt_dec (length G) x); intros LE1 E1; eauto.
+  omega.
+Qed.
+
+Lemma splice_open_commute: forall T n j x,
+(open j (TVar true x) (splice n T)) =
+(splice n (open j (TVar true x) T)).
+Proof.
+  intros. generalize dependent j. induction T; intros; simpl; eauto;
+  try rewrite IHT1; try rewrite IHT2; try rewrite IHT; eauto.
+  destruct b; eauto.
+  case_eq (beq_nat j i); intros E; simpl; eauto.
+Qed.
+
 Lemma index_splice_hi: forall G0 G2 x0 v1 T,
     index x0 (G2 ++ G0) = Some T ->
     length G0 <= x0 ->
@@ -1928,9 +1966,9 @@ Proof.
           (T4::T::GH)) as HGX. {
       simpl. rewrite B. eauto.
     }
-    simpl. change (S (length GH)) with (0 + (S (length GH))).
+    simpl.
     rewrite <- C. rewrite <- D.
-    rewrite splice_open_permute. rewrite splice_open_permute.
+    rewrite splice_open_permute0. rewrite splice_open_permute0.
     rewrite <- HGX.
     apply stp2_splice. simpl. eauto.
 
@@ -2008,6 +2046,149 @@ Lemma stp2_upgrade_gh_mult : forall GH GH' G1 T1 T2 n,
                       stp2 GH G1 T1 T2 n ->
                       stp2 (GH'++GH) G1 T1 T2 n.
 Proof. intros. induction GH'. simpl. eauto. simpl. eapply stp2_upgrade_gh. eauto. Qed. 
+
+Fixpoint splice_tm n (t : tm) {struct t} : tm :=
+  match t with
+    | tvar true i         => tvar true i
+    | tvar false i        => tvar false (splice_var n i)
+    | tobj ds             => tobj (splice_dms n ds)
+    | tapp t1 l t2          => tapp (splice_tm n t1) l (splice_tm n t2)
+  end
+with splice_dm n (d: dm) {struct d} : dm :=
+  match d with
+    | dty T        => dty (splice n T)
+    | dfun T1 T2 t => dfun (splice n T1) (splice n T2) (splice_tm n t)
+  end
+with splice_dms n (ds: dms) {struct ds} : dms :=
+  match ds with
+    | dnil        => dnil
+    | dcons d ds1  => dcons (splice_dm n d) (splice_dms n ds1)
+  end.
+
+Lemma length_splice_dms: forall ds n,
+(length (dms_to_list ds)) = (length (dms_to_list (splice_dms n ds))).
+Proof.
+  intros. induction ds; eauto.
+  simpl. rewrite IHds. eauto.
+Qed.
+
+Lemma hastp_splice_aux: forall ni, (forall GX G0 G1 t1 T1 v1 n,
+   has_type (G1++G0) GX t1 T1 n -> n < ni ->
+   has_type ((map (splice (length G0)) G1) ++ v1::G0) GX
+   (splice_tm (length G0) t1) (splice (length G0) T1) n) /\
+  (forall GX G0 G1 ds1 T1 v1 n,
+   dms_has_type (G1++G0) GX ds1 T1 n -> n < ni ->
+   dms_has_type ((map (splice (length G0)) G1) ++ v1::G0) GX
+   (splice_dms (length G0) ds1) (splice (length G0) T1) n).
+Proof.
+  intro ni. induction ni. split; intros; omega.
+  destruct IHni as [IHT IHD].
+  split; intros; inversion H; subst.
+  - assert (splice (length G0) (substt x T') = substt x T') as A. {
+      eapply closed_splice_idem. eauto. omega.
+    }
+    econstructor. eauto. eauto. eauto. eauto. rewrite A. eauto.
+  - case_eq (le_lt_dec (length G0) x); intros LE E.
+    + econstructor; unfold splice_var; rewrite E.
+      eapply index_splice_hi. eauto. omega.
+      eapply closed_splice. eapply closed_upgrade_gh. eauto. omega.
+    + assert (splice (length G0) T1=T1) as A. {
+        eapply closed_splice_idem. eauto. omega.
+      }
+      econstructor; unfold splice_var; rewrite E.
+      apply index_splice_lo. rewrite A. eauto. omega.
+      rewrite A. eauto.
+  - simpl. destruct b.
+    + assert (splice_tm (length G0) (tvar true x) = tvar true x) as A. {
+        unfold splice_tm. reflexivity.
+      }
+      eapply T_VarPack. rewrite <- A. eapply IHT. eauto. omega.
+      rewrite splice_open_commute. reflexivity.
+      rewrite map_splice_length_inc. eapply closed_splice. eauto.
+    + assert (splice_tm (length G0) (tvar false x) = tvar false (splice_var (length G0) x)) as A. {
+        unfold splice_tm. reflexivity.
+      }
+      eapply T_VarPack. rewrite <- A. eapply IHT. eauto. omega.
+      unfold splice_var.
+      case_eq (le_lt_dec (length G0) x); intros LE E;
+      try solve [rewrite splice_open_permute_lex; eauto; omega];
+      try solve [rewrite splice_open_permute_xgt; eauto; omega].
+      rewrite map_splice_length_inc. eapply closed_splice. eauto.
+  - simpl. destruct b.
+    + assert (splice_tm (length G0) (tvar true x) = tvar true x) as A. {
+        unfold splice_tm. reflexivity.
+      }
+      eapply T_VarUnpack. rewrite <- A.
+      specialize (IHT GX G0 G1 (tvar true x) (TBind T0)). simpl in IHT.
+      eapply IHT. eauto. omega.
+      rewrite splice_open_commute. reflexivity.
+      rewrite map_splice_length_inc. eapply closed_splice. eauto.
+    + assert (splice_tm (length G0) (tvar false x) = tvar false (splice_var (length G0) x)) as A. {
+        unfold splice_tm. reflexivity.
+      }
+      eapply T_VarUnpack. rewrite <- A.
+      specialize (IHT GX G0 G1 (tvar false x) (TBind T0)). simpl in IHT.
+      eapply IHT. eauto. omega.
+      unfold splice_var.
+      case_eq (le_lt_dec (length G0) x); intros LE E;
+      try solve [rewrite splice_open_permute_lex; eauto; omega];
+      try solve [rewrite splice_open_permute_xgt; eauto; omega].
+      rewrite map_splice_length_inc. eapply closed_splice. eauto.
+  - eapply T_Obj.
+    specialize (IHD GX G0 (open 0 (TVar false (length (G1 ++ G0))) T :: G1)).
+    simpl in IHD. eapply IHD. eauto. omega.
+    rewrite map_splice_length_inc. eapply closed_splice. eauto.
+    rewrite map_splice_length_inc. rewrite app_length.
+    rewrite <- splice_open_permute.
+    assert (length G1 + S (length G0)=S (length G1 + length G0)) as A by omega.
+    rewrite A. eauto.
+  - eapply T_App.
+    specialize (IHT GX G0 G1 t0 (TFun l T0 T1)).
+    simpl in IHT. eapply IHT. eauto. omega.
+    eapply IHT. eauto. omega.
+    rewrite map_splice_length_inc. eapply closed_splice. eauto.
+  - simpl. destruct b2.
+    + assert (splice_tm (length G0) (tvar true x2) = tvar true x2) as A. {
+        unfold splice_tm. reflexivity.
+      }
+      eapply T_AppVar.
+      specialize (IHT GX G0 G1 t0 (TFun l T0 T2)).
+      simpl in IHT. eapply IHT. eauto. omega.
+      rewrite <- A. eapply IHT. eauto. omega.
+      rewrite splice_open_commute. reflexivity.
+      rewrite map_splice_length_inc. eapply closed_splice. eauto.
+    + assert (splice_tm (length G0) (tvar false x2) =
+              (tvar false (splice_var (length G0) x2))) as A. {
+        unfold splice_tm. reflexivity.
+      }
+      eapply T_AppVar.
+      specialize (IHT GX G0 G1 t0 (TFun l T0 T2)).
+      simpl in IHT. eapply IHT. eauto. omega.
+      rewrite <- A. eapply IHT. eauto. omega.
+      unfold splice_var.
+      case_eq (le_lt_dec (length G0) x2); intros LE E;
+      try solve [rewrite splice_open_permute_lex; eauto; omega];
+      try solve [rewrite splice_open_permute_xgt; eauto; omega].
+      rewrite map_splice_length_inc. eapply closed_splice. eauto.
+  - eapply T_Sub.
+    eapply IHT. eauto. omega.
+    eapply stp2_splice. eauto.
+  - econstructor.
+  - simpl. eapply D_Mem.
+    eapply IHD. eauto. omega.
+    rewrite map_splice_length_inc. eapply closed_splice. eauto.
+    eauto. eauto. rewrite <- length_splice_dms. eauto.
+  - simpl. eapply D_Abs.
+    eapply IHD. eauto. omega.
+    specialize (IHT GX G0 (T11 :: G1)). simpl in IHT. eapply IHT. eauto. omega.
+    rewrite map_splice_length_inc. repeat rewrite app_length.
+    rewrite <- splice_open_permute.
+    assert (length G1 + S (length G0)=S (length G1 + length G0)) as A by omega.
+    rewrite A. eauto.
+    rewrite map_splice_length_inc. eapply closed_splice. eauto.
+    rewrite map_splice_length_inc. eapply closed_splice. eauto.
+    eauto. rewrite <- length_splice_dms. eauto.
+Qed.
 
 Lemma hastp_upgrade_gh_aux: forall ni,
   (forall T GH G1 t1 T1 n,
